theories/Eq/Shallow.v
@@ -1,0 +1,141 @@
+(** * Shallow equivalence *)
+
+(** Equality under [observe]:
+
+[[
+  observing eq t1 t2 <-> t1.(observe) = t2.(observe)
+]]
+
+  We actually define a more general relation transformer
+  [observing] to lift arbitrary relations through [observe]. *)
+
+From ITree Require Import Core.
+
+From Coq Require Import
+     Classes.RelationClasses
+     Classes.Morphisms
+     Setoids.Setoid
+     Relations.Relations
+     ProofIrrelevance.
+
+(** ** Misc *)
+
+(** Rewrite all heterogeneous equalities with the axiom
+    [inj_pair2 : existT _ T a = existT _ T b -> a = b]. *)
+Ltac auto_inj_pair2 :=
+  repeat (match goal with
+          | [ H : _ |- _ ] => apply inj_pair2 in H
+          end).
+
+Lemma pointwise_relation_fold {A B} {r: relation B} f g :
+  (forall v:A, r (f v) (g v)) -> pointwise_relation _ r f g.
+Proof. red. eauto. Qed.
+
+(**)
+
+(** ** [observing]: Lift relations through [observe]. *)
+Inductive observing {E R1 R2}
+           (eq_ : itree' E R1 -> itree' E R2 -> Prop)
+           (t1 : itree E R1) (t2 : itree E R2) : Prop :=
+| observing_intros :
+    eq_ t1.(observe) t2.(observe) -> observing eq_ t1 t2.
+Hint Constructors observing.
+
+Section observing_relations.
+
+Context {E : Type -> Type} {R : Type}.
+Variable (eq_ : itree' E R -> itree' E R -> Prop).
+
+Global Instance observing_observe :
+  Proper (observing eq_ ==> eq_) (@observe E R).
+Proof. intros ? ? []; cbv; auto. Qed.
+
+Global Instance observing_go : Proper (eq_ ==> observing eq_) (@go E R).
+Proof. cbv; auto. Qed.
+
+Global Instance monotonic_observing eq_' :
+  subrelation eq_ eq_' ->
+  subrelation (observing eq_) (observing eq_').
+Proof. intros ? ? ? []; cbv; eauto. Qed.
+
+Global Instance Equivalence_observing :
+  Equivalence eq_ -> Equivalence (observing eq_).
+Proof.
+  intros []; split; cbv; auto.
+  - intros ? ? []; auto.
+  - intros ? ? ? [] []; eauto.
+Qed.
+
+(* TODO: Ideally, this should subsume [Eq.Eq.itree_eta],
+   see note over there. *)
+Lemma itree_eta_ (t : itree E R) :
+  observing eq t (go (observe t)).
+Proof. auto. Qed.
+
+End observing_relations.
+
+Lemma unfold_bind {E R S}
+      (t : itree E R) (k : R -> itree E S) :
+  observing eq
+    (ITree.bind t k)
+    (ITree.bind_match k (fun t => ITree.bind t k) (observe t)).
+Proof. eauto. Qed.
+
+Instance observing_bind {E R S} :
+  Proper (observing eq ==> eq ==> observing eq) (@ITree.bind E R S).
+Proof.
+  repeat intro; subst.
+  do 2 rewrite unfold_bind; rewrite H.
+  reflexivity.
+Qed.
+
+Lemma ret_bind {E R S} (r : R) (k : R -> itree E S) :
+  observing eq (ITree.bind (Ret r) k) (k r).
+Proof. apply unfold_bind. Qed.
+
+Lemma tau_bind {E R} U t (k: U -> itree E R) :
+  observing eq (ITree.bind (Tau t) k) (Tau (ITree.bind t k)).
+Proof. apply @unfold_bind. Qed.
+
+Lemma vis_bind {E R U V} (e: E V) (ek: V -> itree E U) (k: U -> itree E R) :
+  observing eq
+    (ITree.bind (Vis e ek) k)
+    (Vis e (fun x => ITree.bind (ek x) k)).
+Proof. apply @unfold_bind. Qed.
+
+(** ** [going]: Lift relations through [go]. *)
+
+Inductive going {E R1 R2} (r : itree E R1 -> itree E R2 -> Prop)
+          (ot1 : itree' E R1) (ot2 : itree' E R2) : Prop :=
+| going_intros : r (go ot1) (go ot2) -> going r ot1 ot2.
+Hint Constructors going.
+
+Lemma observing_going {E R1 R2} (eq_ : itree' E R1 -> itree' E R2 -> Prop) ot1 ot2 :
+  going (observing eq_) ot1 ot2 <-> eq_ ot1 ot2.
+Proof.
+  split; auto.
+  intros [[]]; auto.
+Qed.
+
+Section going_relations.
+
+Context {E : Type -> Type} {R : Type}.
+Variable (eq_ : itree E R -> itree E R -> Prop).
+
+Global Instance going_go : Proper (going eq_ ==> eq_) (@go E R).
+Proof. intros ? ? []; auto. Qed.
+
+Global Instance monotonic_going eq_' :
+  subrelation eq_ eq_' ->
+  subrelation (going eq_) (going eq_').
+Proof. intros ? ? ? []; eauto. Qed.
+
+Global Instance Equivalence_going :
+  Equivalence eq_ -> Equivalence (going eq_).
+Proof.
+  intros []; constructor; cbv; eauto.
+  - intros ? ? []; auto.
+  - intros ? ? ? [] []; eauto.
+Qed.
+
+End going_relations.
